mesg_format/contigScript.sml
@@ -5,8 +5,10 @@ open arithmeticTheory listTheory rich_listTheory
      stringTheory combinTheory ASCIInumbersTheory
      numposrepTheory FormalLangTheory;
 
+open bagTheory;  (* For termination of predFn, need to use mlt_list *)
 
 val _ = numLib.prefer_num();
+val _ = overload_on ("++", ``list$APPEND``);
 
 infix byA;
 val op byA = BasicProvers.byA;
@@ -35,8 +37,8 @@ val _ = new_theory "contig";
 Datatype:
   lval = VarName string
        | RecdProj lval string
-       | ArraySub lval exp ;
-
+       | ArraySub lval exp
+  ;
   exp = Loc lval
       | numLit num
       | ConstName string
@@ -50,11 +52,11 @@ Datatype:
        | Bnot bexp
        | Bor  bexp bexp
        | Band bexp bexp
-       | Beq  exp exp
-       | Blt  exp exp
-       | Bgtr exp exp
-       | Bleq exp exp
-       | Bgeq exp exp
+       | Beq exp exp
+       | Blt exp exp
+       | Bgt exp exp
+       | Ble exp exp
+       | Bge exp exp
 End
 
 Datatype:
@@ -76,7 +78,6 @@ Datatype:
          | Array contig exp
          | Union ((bexp # contig) list)
 End
-
 
 (*---------------------------------------------------------------------------*)
 (* comparison functions on lvals and exps                                    *)
@@ -124,11 +125,31 @@ Definition evalExp_def :
    (case lookup lval_compare lval lvalMap
      of SOME s => valueFn s
       | NONE => ARB) /\
- evalExp E (numLit n) = n /\
- evalExp E (Add e1 e2) = (evalExp E e1 + evalExp E e2) /\
+ evalExp E (numLit n)   = n /\
+ evalExp E (Add e1 e2)  = (evalExp E e1 + evalExp E e2) /\
  evalExp E (Mult e1 e2) = (evalExp E e1 * evalExp E e2)
 End
 
+
+(*---------------------------------------------------------------------------*)
+(* Boolean expression evaluation                                             *)
+(*---------------------------------------------------------------------------*)
+
+Definition evalBexp_def :
+ (evalBexp E (boolLit b)   = b) /\
+ (evalBexp (lvalMap,valueFn) (BLoc lval) =
+   (case lookup lval_compare lval lvalMap
+     of SOME s => ~(valueFn s = 0n)
+      | NONE => ARB)) /\
+ (evalBexp E (Bnot b)     = ~evalBexp E b) /\
+ (evalBexp E (Bor b1 b2)  = (evalBexp E b1 \/ evalBexp E b2)) /\
+ (evalBexp E (Band b1 b2) = (evalBexp E b1 /\ evalBexp E b2)) /\
+ (evalBexp E (Beq e1 e2)  = (evalExp E e1 = evalExp E e2))  /\
+ (evalBexp E (Blt e1 e2)  = (evalExp E e1 < evalExp E e2))  /\
+ (evalBexp E (Bgt e1 e2)  = (evalExp E e1 > evalExp E e2))  /\
+ (evalBexp E (Ble e1 e2)  = (evalExp E e1 <= evalExp E e2)) /\
+ (evalBexp E (Bge e1 e2)  = (evalExp E e1 >= evalExp E e2))
+End
 
 (*---------------------------------------------------------------------------*)
 (* Location completion                                                       *)
@@ -148,6 +169,153 @@ Definition path_prefixes_def :
   path_prefixes (ArraySub arr dim) = ArraySub arr dim :: path_prefixes arr
 End
 
+Definition optFirst_def :
+  optFirst f [] = NONE /\
+  optFirst f (h::t) =
+    case f h
+     of NONE => optFirst f t
+      | SOME x => SOME h
+End
 
+(*---------------------------------------------------------------------------*)
+(* Does a partial lval resolve to something in the lvalMap? This is a kind   *)
+(* of dynamic scoping.                                                       *)
+(*---------------------------------------------------------------------------*)
+
+Definition resolve_lval_def :
+ resolve_lval lvalMap path lval =
+   let prefixes = path_prefixes path ;
+       prospects = MAP (combin$C lval_append lval) prefixes ++ [lval] ;
+   in THE (optFirst (\p. lookup lval_compare p lvalMap) prospects)
+End
+
+Definition resolveExp_def:
+ resolveExp lvmap p (Loc lval) = Loc(resolve_lval lvmap p lval) /\
+ resolveExp lvmap p (Add e1 e2) = Add (resolveExp lvmap p e1) (resolveExp lvmap p e2) /\
+ resolveExp lvmap p (Mult e1 e2) = Mult (resolveExp lvmap p e1) (resolveExp lvmap p e2) /\
+ resolveExp lvmap p (numLit n) = numLit n  /\
+ resolveExp lvmap p (ConstName s) = ConstName s
+End
+
+Definition resolveBexp_def :
+ resolveBexp lvmap p (boolLit b) = boolLit b /\
+ resolveBexp lvmap p (BLoc lval) = BLoc (resolve_lval lvmap p lval) /\
+ resolveBexp lvmap p (Bnot b)    = Bnot (resolveBexp lvmap p b) /\
+ resolveBexp lvmap p (Bor b1 b2) = Bor (resolveBexp lvmap p b1) (resolveBexp lvmap p b2) /\
+ resolveBexp lvmap p (Band b1 b2) = Band (resolveBexp lvmap p b1) (resolveBexp lvmap p b2) /\
+ resolveBexp lvmap p (Beq e1 e2) = Beq (resolveExp lvmap p e1) (resolveExp lvmap p e2) /\
+ resolveBexp lvmap p (Blt e1 e2) = Blt (resolveExp lvmap p e1) (resolveExp lvmap p e2) /\
+ resolveBexp lvmap p (Bgt e1 e2) = Bgt (resolveExp lvmap p e1) (resolveExp lvmap p e2) /\
+ resolveBexp lvmap p (Ble e1 e2) = Ble (resolveExp lvmap p e1) (resolveExp lvmap p e2) /\
+ resolveBexp lvmap p (Bge e1 e2) = Bge (resolveExp lvmap p e1) (resolveExp lvmap p e2)
+End
+
+(*---------------------------------------------------------------------------*)
+(* break off a prefix of a string                                            *)
+(*---------------------------------------------------------------------------*)
+
+Definition tdrop_def:
+ tdrop 0 list acc = SOME (REVERSE acc, list) /\
+ tdrop n [] acc = NONE /\
+ tdrop (SUC n) (h::t) acc = tdrop n t (h::acc)
+End
+
+Definition take_drop_def :
+  take_drop n list = tdrop n list []
+End
+
+Definition upto_def:
+ upto lo hi = if lo > hi then [] else lo::upto (lo+1) hi
+Termination
+ WF_REL_TAC `measure (\(a,b). b+1n - a)`
+End
+
+Theorem upto_thm :
+ !lo hi. set(upto lo hi) = {n | lo <= n /\ n <= hi}
+Proof
+ recInduct upto_ind
+  >> rw_tac list_ss []
+  >> rw_tac list_ss [Once upto_def]
+  >> fs[]
+  >> rw [pred_setTheory.EXTENSION]
+QED
+
+(*---------------------------------------------------------------------------*)
+(* Size of a contig. The system-generated contig_size goes through a lot of  *)
+(* other types, including strings (field names) and they shouldn't be counted*)
+(* because field name size shouldn't count in the size of the expression.    *)
+(*---------------------------------------------------------------------------*)
+
+val contig_size_def = fetch "-" "contig_size_def";
+
+val _ = add_cong list_size_cong;
+
+Definition csize_def :
+  (csize FAIL            = 0) /\
+  (csize (Basic a)       = 0) /\
+  (csize (Recd fields)   = 1 + list_size (\(a,c). csize  c) fields) /\
+  (csize (Array c dim)   = 1 + csize c) /\
+  (csize (Union choices) = 1 + list_size (\(b,c). csize c) choices)
+Termination
+  WF_REL_TAC `measure contig_size`
+  >> rw_tac list_ss [contig_size_def]
+   >- (Induct_on `choices`
+        >> rw_tac list_ss [contig_size_def]
+        >> full_simp_tac list_ss [contig_size_def])
+   >- (Induct_on `fields`
+        >> rw_tac list_ss [contig_size_def]
+        >> full_simp_tac list_ss [contig_size_def])
+End
+
+Triviality list_size_append :
+ !L1 L2 f. list_size f (L1 ++ L2) = (list_size f L1 + list_size f L2)
+Proof
+ Induct_on `L1` >> rw_tac list_ss [list_size_def]
+QED
+
+(*---------------------------------------------------------------------------*)
+(* contig-specified predicate on strings.                                    *)
+(*---------------------------------------------------------------------------*)
+
+Definition predFn_def :
+ predFn (atomWidths,valueFn) (worklist,s,theta) =
+  case worklist
+   of [] => T
+    | (path,FAIL)::t => F
+    | (path,Basic a)::t =>
+        (case take_drop (atomWidths a) s
+           of NONE => F
+            | SOME (segment,rst) =>
+              predFn (atomWidths,valueFn)
+                     (t, rst, insert lval_compare path segment theta))
+   | (path,Recd fields)::t =>
+      let fieldFn (fName,c) = (RecdProj path fName,c)
+      in predFn (atomWidths,valueFn) (MAP fieldFn fields ++ t,s,theta)
+   | (path,Array c exp)::t =>
+      let exp' = resolveExp theta path exp;
+          dim  = evalExp (theta,valueFn) exp';
+          indexFn n = (ArraySub path (numLit n),c)
+      in predFn (atomWidths,valueFn)
+                (MAP indexFn (upto 0 (dim - 1)) ++ t,s,theta)
+   | (path,Union choices)::t =>
+       let choiceFn (bexp,c) =
+             evalBexp (theta,valueFn)
+                      (resolveBexp theta path bexp)
+       in case FILTER choiceFn choices
+           of [(_,c)] => predFn (atomWidths,valueFn) ((path,c)::t,s,theta)
+            | otherwise => F
+Termination
+ WF_REL_TAC `inv_image (mlt_list (measure (csize o SND))) (FST o SND)`
+   >> rw [APPEND_EQ_SELF]
+   >> rw [csize_def]
+   >> fs [MEM_MAP,MEM_SPLIT]
+   >- (Cases_on `y` >> fs[list_size_append,list_size_def])
+   >- fs [FILTER_EQ_CONS,list_size_append,list_size_def]
+End
+
+
+(*
+fun wellformed E contig s = predFn E ([(VarName"root",contig)],s,empty_lvalMap);
+*)
 
 val _ = export_theory();
